

CS70 HW 12

March 15, 2021

1 Safeway Monopoly Cards

- (a) I have no idea about the solution this question. The hint must be something about Collector Coupon Problem and the Expectation and Variance of Geometric(p). But i can't see the connection.

$$\begin{aligned} \text{Var}(X) &= \text{Var}\left(\sum_{i=1}^n X_i\right) \\ &= \sum_{i=1}^n \text{Var}(X_i) && \text{independence} \\ &= \sum_{i=1}^n \frac{1 - \frac{n-i+1}{n}}{\left(\frac{n-i+1}{n}\right)^2} && p = \frac{n-i+1}{n} \\ &= \sum_{j=1}^n \frac{1 - j/n}{(j/n)^2} && n-i+1 = n \rightarrow 1 \\ &= \sum_{j=1}^n \frac{n9n-j)}{j^2} \\ &= \sum_{j=1}^n n^2 j^{-2} - n \sum_{j=1}^n i^{-1} \\ &= n^2 \sum_{j=1}^n j^{-2} - E(X) \end{aligned}$$

2 Geometric Distribution

- (a) From the description, we can infer that $X = X_1 \cup X_2$. Thus $P(X = 1) = P(X_1 = 1 \cap X_2 = 1) = P(X_1 = 1) + P(X_2 = 1) - P(X_1 = 1 \cap X_2 = 1) = p_1 + p_2 - p_1 p_2$.

Therefore, it's also a geometric distribution with parameter $p' = p_1 + p_2 - p_1p_2$.

It seems that it's not that simple. We should consider this problem more carefully. And $X \neq X_1 \cup X_2$ but $X = \min\{X_1, X_2\}$.

Here the best way to solve this is that to show the tail probability is Geometric Contribution.

$$\begin{aligned} Pr(X \geq k) &= Pr(\min\{X_1, X_2\} \geq k) \\ &= Pr(X_1 \geq k \cap X_2 \geq k) \\ &= (1 - p_1)^{k-1} * (1 - p_2)^{k-1} \\ &= (1 - (p_1 + p_2 - p_1p_2))^{k-1} \end{aligned}$$

Thus $p' = p_1 + p_2 - p_1p_2$.

- (b) From the distribution of X , we can know that the probability for the first person to find is that

$$\sum_{i=0}^{\infty} (1 - p')^{2i} \cdot p' = \frac{p'}{1 - (1 - p')^2}$$

where $p' = p_1 + p_2 - p_1p_2$.

3 Geometric and Poisson

- (a)

$$\begin{aligned} Pr(X > Y) &= \sum_{x=1}^{\infty} \sum_{y=0}^{x-1} \frac{\lambda^y}{y!} e^{-\lambda} \cdot (1 - p)^{x-1} p \\ &= \sum_{y=0}^{\infty} \sum_{x=y+1}^{\infty} \frac{\lambda^y}{y!} e^{-\lambda} \cdot (1 - p)^{x-1} p \\ &= \sum_{y=0}^{\infty} \frac{\lambda^y}{y!} e^{-\lambda} \cdot \sum_{x=y+1}^{\infty} (1 - p)^{x-1} p \\ &= \sum_{y=0}^{\infty} \frac{\lambda^y}{y!} e^{-\lambda} \cdot (1 - p)^y \\ &= \frac{\sum_{y=0}^{\infty} \frac{[\lambda(1-p)]^y}{y!} e^{-\lambda(1-p)}}{e^{1-p}} \\ &= \frac{1}{e^{1-p}} = e^{p-1}. \end{aligned}$$

We are almost right, but a simple mistake here. The last two steps, it should be

$$\begin{aligned} Pr(X > Y) &= \frac{\sum_{y=0}^{\infty} \frac{[\lambda(1-p)]^y}{y!} e^{-\lambda(1-p)}}{e^p} \\ &= \frac{1}{e^{\lambda p}} = e^{-\lambda p} \end{aligned}$$

(b) Since $\max\{X, Y\} \geq X$, we infer that $P(\max\{X, Y\} \geq X) = 1$.

(c) Since $\max\{X, Y\} \geq Y$ and now we want $\max\{X, Y\} \leq Y$, we can infer that $\max\{X, Y\} = Y$, which is same as $P(X \leq Y) = 1 - P(X > Y) = 1 - e^{-\lambda p}$.

Because of part(a), the right answer shall be $1 - e^{-\lambda p}$.

4 Darts

(a) $f_X(x) = \exp(-x)$. First we check that the integral is 1.

$$\int_0^{\infty} e^{-x} dx = \frac{e^{-x}}{-1} \Big|_{x=0}^{x=\infty} = 1$$

Then $\Pr(\text{dart will stay within the board}) =$

$$\int_0^4 e^{-x} dx = \frac{e^{-x}}{-1} \Big|_{x=0}^{x=4} = 1 - e^{-4}.$$

(b) $\Pr(\text{within 1 unit} \mid \text{within 4 unit}) = \frac{\Pr(\text{within 1 unit})}{\Pr(\text{within 4 unit})} =$

$$\frac{\int_0^1 e^{-x} dx}{\int_0^4 e^{-x} dx} = \frac{1 - e^{-1}}{1 - e^{-4}}$$

(c) $\Pr(\text{Score}) =$

$$\begin{cases} 1 - e^{-1} & 0 \leq x \leq 1, S = 4 \\ e^{-1} - e^{-2} & 1 \leq x \leq 2, S = 3 \\ e^{-2} - e^{-3} & 2 \leq x \leq 3, S = 2 \\ e^{-3} - e^{-4} & 3 \leq x \leq 4, S = 1 \end{cases}$$

Thus we have the $E(S) =$

$$4(1 - e^{-1}) + 3(e^{-1} - e^{-2}) + 2(e^{-2} - e^{-3}) + 1(e^{-3} - e^{-4}) = 4 - \sum_{i=1}^4 e^{-i}$$

5 Exponential Practice

(a) We can compute as following:

$$\begin{aligned}
 F_Y(y) &= \int_0^y \int_0^{c-x_1} \lambda e^{-\lambda x_1} \lambda e^{-\lambda x_2} dx_1 dx_2 \\
 &= \int_0^y e^{-\lambda x_1} \cdot \int_0^{c-x_1} \lambda e^{-\lambda x_2} dx_2 dx_1 \\
 &= \int_0^y e^{-\lambda x_1} \cdot \frac{e^{-\lambda x_2}}{-\lambda} \Big|_0^{c-x_1} dx_1 \\
 &= \int_0^y e^{-\lambda x_1} \cdot (1 - e^{-\lambda(c-x_1)}) dx_1 \\
 &= \int_0^y e^{-\lambda x_1} dx_1 - \int_0^y \lambda e^{-\lambda y} dx_1 \\
 &= 1 - e^{-\lambda y} - \lambda y e^{-\lambda y}
 \end{aligned}$$

Then differentiate it, we obtain

$$\begin{aligned}
 f_Y(y) &= \lambda e^{-\lambda y} - [\lambda e^{-\lambda y} - \lambda^2 y e^{-\lambda y}] \\
 &= \lambda^2 y e^{-\lambda y}
 \end{aligned}$$

(b)

$$\begin{aligned}
 \frac{Pr(X_1 \leq x \cap x_1 + x_2 = t)}{Pr(x_1 + x_2 = t)} &= \frac{\text{Same as part(a)}}{f_T(t) dt} \\
 &= \frac{1 - e^{-\lambda x} - \lambda x e^{-\lambda x}}{\lambda^2 t e^{-\lambda t} dt} \\
 &= \text{I don't know the next} \\
 &= \text{now maybe I know} \\
 &= \text{this is wrong}
 \end{aligned}$$

$$\begin{aligned}
 \frac{Pr(X_1 \leq x \cap x_1 + x_2 = t)}{Pr(x_1 + x_2 = t)} &= \frac{\int_0^x \lambda^2 t e^{-\lambda t} dt dx}{\int_0^t \lambda^2 t e^{-\lambda t} dt dx} \\
 &= \frac{x \lambda^2 t e^{-\lambda t} dt}{t \lambda^2 t e^{-\lambda t} dt} \\
 &= \frac{x}{t}
 \end{aligned}$$

Therefore, pdf of X_1 conditioned on $X_1 + X_2 = t$ is $\frac{1}{t}$.

6 Uniform Means

(a) By tail sum formula, $E(X) = \int_0^\infty P(X > x) dx$, we have

$$\begin{aligned} E(Y) &= \int_0^\infty P(Y > y) dy \\ &= \int_0^1 P(Y > y) dy \\ &= \int_0^1 \left(\frac{1-y}{1}\right)^n dy \\ &= - \int_0^1 \left(\frac{1-y}{y}\right)^n d(1-y) \\ &= - \left. \frac{(1-y)^{n+1}}{n+1} \right|_0^1 \\ &= \frac{1}{n+1} \end{aligned}$$

(b) Find the CDF, $F_Z(z) = Pr(Z \leq z) = \left(\frac{z}{1}\right)^n = z^n$. Therefore, $f_Z(z) = n \cdot z^{n-1}$.

$$\begin{aligned} E(Z) &= \int_0^1 zn \cdot z^{n-1} dz \\ &= n \cdot \int_0^1 z^n dz \\ &= n \cdot \left. \frac{z^{n+1}}{n+1} \right|_0^1 \\ &= \frac{n}{n+1} \end{aligned}$$